Verify saturn/mpsc_queue_1.

theories/saturn/mpsc_queue_1.v
@@ -1,16 +1,24 @@
 From zoo Require Import
   prelude.
+From zoo.common Require Import
+  list.
+From zoo.iris.base_logic Require Import
+  lib.mono_list
+  lib.twins.
 From zoo.language Require Import
   notations
   diaframe.
 From zoo.std Require Import
   option
-  node2_chain.
+  node2_schain.
 From zoo.saturn Require Export
   base.
 From zoo Require Import
   options.
 
+Implicit Types b au_empty au_nonempty : bool.
+Implicit Types l front node back new_back : location.
+Implicit Types hist past nodes : list location.
 Implicit Types v t : val.
 Implicit Types vs : list val.
 
@@ -38,23 +46,23 @@ Definition mpsc_queue_is_empty : val :=
     if: "node'" = () then (
       ifnot: Cas "node".[node2_next] () "new_back" then (
         Yield ;;
-        "mpsc_queue_do_push" "node'" "new_back"
+        "mpsc_queue_do_push" "node" "new_back"
       )
     ) else (
       "mpsc_queue_do_push" "node'" "new_back"
     ).
 #[local] Definition mpsc_queue_fix_back : val :=
-  rec: "mpsc_queue_fix_back" "t" "new_back" :=
-    let: "back" := "t".{back} in
+  rec: "mpsc_queue_fix_back" "t" "back" "new_back" :=
     if: "new_back".{node2_next} = () and ~ Cas "t".[back] "back" "new_back" then (
       Yield ;;
-      "mpsc_queue_fix_back" "t" "new_back"
+      "mpsc_queue_fix_back" "t" "t".{back} "new_back"
     ).
 Definition mpsc_queue_push : val :=
   λ: "t" "v",
     let: "new_back" := node2_create "v" () in
-    mpsc_queue_do_push "t".{back} "new_back" ;;
-    mpsc_queue_fix_back "t" "new_back".
+    let: "back" := "t".{back} in
+    mpsc_queue_do_push "back" "new_back" ;;
+    mpsc_queue_fix_back "t" "back" "new_back".
 
 Definition mpsc_queue_pop : val :=
   λ: "t",
@@ -69,47 +77,180 @@ Definition mpsc_queue_pop : val :=
     ).
 
 Class MpscQueueG Σ `{zoo_G : !ZooG Σ} := {
+  #[local] mpsc_queue_G_history_G :: MonoListG Σ location ;
+  #[local] mpsc_queue_G_model_G :: TwinsG Σ (leibnizO (list val)) ;
 }.
 
 Definition mpsc_queue_Σ := #[
+  mono_list_Σ location ;
+  twins_Σ (leibnizO (list val))
 ].
 #[global] Instance subG_mpsc_queue_Σ Σ `{zoo_G : !ZooG Σ} :
   subG mpsc_queue_Σ Σ →
   MpscQueueG Σ.
 Proof.
+  solve_inG.
 Qed.
 
 Section mpsc_queue_G.
   Context `{mpsc_queue_G : MpscQueueG Σ}.
 
-  Definition mpsc_queue_inv t (ι : namespace) : iProp Σ.
-  Proof. Admitted.
+  Record mpsc_queue_meta := {
+    mpsc_queue_meta_history : gname ;
+    mpsc_queue_meta_model : gname ;
+  }.
 
-  Definition mpsc_queue_model t vs : iProp Σ.
-  Proof. Admitted.
+  #[local] Instance mpsc_queue_meta_eq_dec : EqDecision mpsc_queue_meta :=
+    ltac:(solve_decision).
+  #[local] Instance mpsc_queue_meta_countable :
+    Countable mpsc_queue_meta.
+  Proof.
+    pose encode γ := (
+      γ.(mpsc_queue_meta_history),
+      γ.(mpsc_queue_meta_model)
+    ).
+    pose decode := λ '(γ_history, γ_model), {|
+      mpsc_queue_meta_history := γ_history ;
+      mpsc_queue_meta_model := γ_model ;
+    |}.
+    refine (inj_countable' encode decode _). intros []. done.
+  Qed.
 
-  Definition mpsc_queue_consumer t : iProp Σ.
-  Proof. Admitted.
+  #[local] Definition mpsc_queue_history_auth' γ_history hist :=
+    mono_list_auth γ_history (DfracOwn 1) hist.
+  #[local] Definition mpsc_queue_history_auth γ hist :=
+    mpsc_queue_history_auth' γ.(mpsc_queue_meta_history) hist.
+  #[local] Definition mpsc_queue_history_elem γ i node :=
+    mono_list_elem γ.(mpsc_queue_meta_history) i node.
+
+  #[local] Definition mpsc_queue_model₁' γ_model vs :=
+    twins_twin1 γ_model (DfracOwn 1) vs.
+  #[local] Definition mpsc_queue_model₁ γ vs :=
+    mpsc_queue_model₁' γ.(mpsc_queue_meta_model) vs.
+  #[local] Definition mpsc_queue_model₂' γ_model vs :=
+    twins_twin2 γ_model vs.
+  #[local] Definition mpsc_queue_model₂ γ vs :=
+    mpsc_queue_model₂' γ.(mpsc_queue_meta_model) vs.
+
+  #[local] Definition mpsc_queue_inv_inner l γ : iProp Σ :=
+    ∃ hist past front nodes back vs,
+    ⌜hist = past ++ front :: nodes⌝ ∗
+    ⌜back ∈ hist⌝ ∗
+    l.[front] ↦{#1/4} #front ∗
+    l.[back] ↦ #back ∗
+    node2_schain hist () ∗
+    ([∗ list] node; v ∈ nodes; vs, node.[node2_data] ↦ v) ∗
+    mpsc_queue_history_auth γ hist ∗
+    mpsc_queue_model₂ γ vs.
+  Definition mpsc_queue_inv t ι : iProp Σ :=
+    ∃ l γ,
+    ⌜t = #l⌝ ∗
+    meta l nroot γ ∗
+    inv ι (mpsc_queue_inv_inner l γ).
+
+  Definition mpsc_queue_model t vs : iProp Σ :=
+    ∃ l γ,
+    ⌜t = #l⌝ ∗
+    meta l nroot γ ∗
+    mpsc_queue_model₁ γ vs.
+
+  Definition mpsc_queue_consumer t : iProp Σ :=
+    ∃ l front,
+    ⌜t = #l⌝ ∗
+    l.[front] ↦{#3/4} #front.
 
   #[global] Instance mpsc_queue_model_timeless t vs :
     Timeless (mpsc_queue_model t vs).
   Proof.
-  Admitted.
+    apply _.
+  Qed.
   #[global] Instance mpsc_queue_consumer_timeless t :
     Timeless (mpsc_queue_consumer t ).
   Proof.
-  Admitted.
+    apply _.
+  Qed.
   #[global] Instance mpsc_queue_inv_persistent t ι :
     Persistent (mpsc_queue_inv t ι).
   Proof.
-  Admitted.
+    apply _.
+  Qed.
+
+  #[local] Lemma mpsc_queue_history_alloc front :
+    ⊢ |==>
+      ∃ γ_hist,
+      mpsc_queue_history_auth' γ_hist [front].
+  Proof.
+    apply mono_list_alloc.
+  Qed.
+  #[local] Lemma mpsc_queue_history_elem_get {γ hist} i node :
+    hist !! i = Some node →
+    mpsc_queue_history_auth γ hist ⊢
+    mpsc_queue_history_elem γ i node.
+  Proof.
+    setoid_rewrite mono_list_lb_get. apply mono_list_elem_get.
+  Qed.
+  #[local] Lemma mpsc_queue_history_agree γ hist i node :
+    mpsc_queue_history_auth γ hist -∗
+    mpsc_queue_history_elem γ i node -∗
+    ⌜hist !! i = Some node⌝.
+  Proof.
+    apply mono_list_lookup.
+  Qed.
+  #[local] Lemma mpsc_queue_history_update {γ hist} node :
+    mpsc_queue_history_auth γ hist ⊢ |==>
+    mpsc_queue_history_auth γ (hist ++ [node]).
+  Proof.
+    apply mono_list_update_app.
+  Qed.
+
+  #[local] Lemma mpsc_queue_model_alloc :
+    ⊢ |==>
+      ∃ γ_model,
+      mpsc_queue_model₁' γ_model [] ∗
+      mpsc_queue_model₂' γ_model [].
+  Proof.
+    apply twins_alloc'.
+  Qed.
+  #[local] Lemma mpsc_queue_model_agree γ model1 model2 :
+    mpsc_queue_model₁ γ model1 -∗
+    mpsc_queue_model₂ γ model2 -∗
+    ⌜model1 = model2⌝.
+  Proof.
+    apply: twins_agree_L.
+  Qed.
+  #[local] Lemma mpsc_queue_model_update {γ vs1 vs2} vs :
+    mpsc_queue_model₁ γ vs1 -∗
+    mpsc_queue_model₂ γ vs2 ==∗
+      mpsc_queue_model₁ γ vs ∗
+      mpsc_queue_model₂ γ vs.
+  Proof.
+    apply twins_update'.
+  Qed.
+
+  #[local] Lemma mpsc_queue_inv_inner_history_elem ι l γ front :
+    inv ι (mpsc_queue_inv_inner l γ) -∗
+    l.[front] ↦{#3/4} #front ={⊤}=∗
+      ∃ i,
+      l.[front] ↦{#3/4} #front ∗
+      mpsc_queue_history_elem γ i front.
+  Proof.
+    iIntros "#Hinv Hl_front_1".
+    iInv "Hinv" as "(%hist & %past & %_front & %nodes & %back & %vs & >%Hhist & >%Hback & >Hl_front_2 & Hl_back & Hhist & Hnodes & >Hhistory_auth & Hmodel₂)".
+    iDestruct (pointsto_agree with "Hl_front_1 Hl_front_2") as %[= <-].
+    iDestruct (mpsc_queue_history_elem_get (length past) front with "Hhistory_auth") as "#Hhistory_elem".
+    { rewrite Hhist list_lookup_middle //. }
+    iSplitR "Hl_front_1". { repeat iExists _. iSteps. }
+    iSteps.
+  Qed.
 
   Lemma mpsc_queue_consumer_exclusive t :
     mpsc_queue_consumer t -∗
     mpsc_queue_consumer t -∗
     False.
   Proof.
-  Admitted.
+    iIntros "(%l & %front & -> & Hl_front_1) (%_l & %_front & %Heq & Hl_front_2)". injection Heq as <-.
+    iDestruct (pointsto_frac_ne with "Hl_front_1 Hl_front_2") as %?; naive_solver.
+  Qed.
 
   Lemma mpsc_queue_create_spec ι :
     {{{ True }}}
@@ -121,7 +262,388 @@ Section mpsc_queue_G.
       mpsc_queue_consumer t
     }}}.
   Proof.
-  Admitted.
+    iIntros "%Φ _ HΦ".
+
+    wp_rec.
+
+    wp_apply (node2_create_spec with "[//]") as (front) "Hfront".
+    wp_record l as "Hmeta" "(Hl_front & Hl_back & _)".
+    iEval (rewrite -Qp.three_quarter_quarter) in "Hl_front".
+    iDestruct "Hl_front" as "(Hl_front_1 & Hl_front_2)".
+
+    iMod mpsc_queue_history_alloc as "(%γ_history & Hhistory_auth)".
+    iMod mpsc_queue_model_alloc as "(%γ_model & Hmodel₁ & Hmodel₂)".
+
+    pose γ := {|
+      mpsc_queue_meta_history := γ_history ;
+      mpsc_queue_meta_model := γ_model ;
+    |}.
+
+    iMod (meta_set _ _ γ with "Hmeta") as "#Hmeta"; first done.
+
+    iApply "HΦ".
+    iSplitR "Hmodel₁ Hl_front_1"; last iSteps.
+    iStep 2. iApply inv_alloc.
+    iExists [front], [], front, [], front, []. iFrame. iSteps.
+    rewrite elem_of_list_singleton //.
+  Qed.
+
+  #[local] Lemma mpsc_queue_front_spec l γ ι :
+    {{{
+      inv ι (mpsc_queue_inv_inner l γ)
+    }}}
+      !#l.[front]
+    {{{ front i,
+      RET #front;
+      mpsc_queue_history_elem γ i front
+    }}}.
+  Proof.
+    iIntros "%Φ #Hinv HΦ".
+
+    iInv "Hinv" as "(%hist & %past & %front & %nodes & %back & %vs & >%Hhist & >%Hback & Hl_front & Hl_back & Hhist & Hnodes & Hhistory_auth & Hmodel₂)".
+    wp_load.
+    iDestruct (mpsc_queue_history_elem_get _ front with "Hhistory_auth") as "#Hhistory_elem".
+    { rewrite Hhist list_lookup_middle //. }
+    iSplitR "HΦ". { repeat iExists _. iSteps. }
+    iSteps.
+  Qed.
+
+  #[local] Lemma mpsc_queue_back_spec l γ ι :
+    {{{
+      inv ι (mpsc_queue_inv_inner l γ)
+    }}}
+      !#l.[back]
+    {{{ back i,
+      RET #back;
+      mpsc_queue_history_elem γ i back
+    }}}.
+  Proof.
+    iIntros "%Φ #Hinv HΦ".
+
+    iInv "Hinv" as "(%hist & %past & %front & %nodes & %back & %vs & >%Hhist & >%Hback & Hl_front & Hl_back & Hhist & Hnodes & Hhistory_auth & Hmodel₂)".
+    wp_load.
+    pose proof Hback as (i & Hlookup)%elem_of_list_lookup.
+    iDestruct (mpsc_queue_history_elem_get with "Hhistory_auth") as "#Hhistory_elem_back"; first done.
+    iSplitR "HΦ". { repeat iExists _. iSteps. }
+    iSteps.
+  Qed.
+
+  #[local] Lemma mpsc_queue_node2_next_spec_strong au_empty au_nonempty TB β x_empty x_nonempty Ψ l γ ι i node :
+    {{{
+      meta l nroot γ ∗
+      inv ι (mpsc_queue_inv_inner l γ) ∗
+      mpsc_queue_history_elem γ i node ∗
+      ( if negb au_empty && negb au_nonempty then True else
+        l.[front] ↦{#3/4} #node ∗
+        atomic_update (TA := [tele vs]) (TB := TB) (⊤ ∖ ↑ι) ∅ (tele_app $ mpsc_queue_model #l) β Ψ
+      ) ∗
+      ( if negb au_empty then True else
+        mpsc_queue_model #l [] -∗
+        β [tele_arg []] x_empty
+      ) ∗
+      ( if negb au_nonempty then True else
+        ∀ vs,
+        ⌜vs ≠ []⌝ -∗
+        mpsc_queue_model #l vs -∗
+        β (TeleArgCons vs ()) x_nonempty
+      )
+    }}}
+      !#node.[node2_next]
+    {{{ res,
+      RET res;
+      ( ⌜res = ()%V⌝ ∗
+        if negb au_empty then True else
+          l.[front] ↦{#3/4} #node ∗
+          Ψ [tele_arg []] x_empty
+      ) ∨ (
+        ∃ node',
+        ⌜res = #node'⌝ ∗
+        mpsc_queue_history_elem γ (S i) node' ∗
+        if negb au_empty then True else
+          l.[front] ↦{#3/4} #node ∗
+          if au_nonempty then
+            ∃ vs, Ψ (TeleArgCons vs ()) x_nonempty
+          else
+            atomic_update (TA := [tele vs]) (TB := TB) (⊤ ∖ ↑ι) ∅ (tele_app $ mpsc_queue_model #l) β Ψ
+      )
+    }}}.
+  Proof.
+    iIntros "%Φ (#Hmeta & #Hinv & #Hhistory_elem & HΨ & Hβ_empty & Hβ_nonempty) HΦ".
+
+    iInv "Hinv" as "(%hist & %past & %front & %nodes & %back & %vs & >%Hhist & >%Hback & Hl_front_2 & Hl_back & Hhist & Hnodes & >Hhistory_auth & Hmodel₂)".
+    iDestruct (mpsc_queue_history_agree with "Hhistory_auth Hhistory_elem") as %Hlookup.
+    iDestruct (node2_schain_lookup with "Hhist") as "(Hnode & Hhist)"; first done.
+    wp_load.
+    iDestruct ("Hhist" with "Hnode ") as "Hhist".
+    destruct (hist !! S i) as [node' |] eqn:Hlookup'; simpl.
+
+    - iDestruct (mpsc_queue_history_elem_get (S i) with "Hhistory_auth") as "#Hhistory_elem'"; first done.
+      destruct au_nonempty.
+
+      + rewrite andb_false_r /=.
+        iDestruct "HΨ" as "(Hl_front_1 & HΨ)".
+        iDestruct (pointsto_agree with "Hl_front_1 Hl_front_2") as %[= ->].
+        iMod "HΨ" as "(%_vs & (%_l & %_γ & %Heq & #_Hmeta & Hmodel₁) & _ & HΨ)". injection Heq as <-.
+        iDestruct (meta_agree with "Hmeta _Hmeta") as %<-. iClear "_Hmeta".
+        iDestruct (mpsc_queue_model_agree with "Hmodel₁ Hmodel₂") as %->.
+        iDestruct ("Hβ_nonempty" with "[#] [Hmodel₁]") as "Hβ"; [| iSteps |].
+        { iAssert ⌜length past = i⌝%I as %Hpast_length.
+          { iDestruct (node2_schain_NoDup with "Hhist") as %Hnodup.
+            iPureIntro. eapply NoDup_lookup; try done.
+            rewrite Hhist list_lookup_middle //.
+          }
+          rewrite -length_zero_iff_nil.
+          iDestruct (big_sepL2_length with "Hnodes") as %<-.
+          iIntros "%Hnodes_length". iPureIntro.
+          apply (f_equal length) in Hhist as Hhist_length.
+          rewrite app_length /= in Hhist_length.
+          apply lookup_lt_Some in Hlookup'.
+          lia.
+        }
+        iMod ("HΨ" $! x_nonempty with "Hβ") as "HΨ".
+        iSplitR "Hl_front_1 HΨ HΦ". { repeat iExists _. iSteps. }
+        destruct au_empty; iSteps.
+
+      + iSplitR "HΨ HΦ". { repeat iExists _. iSteps. }
+        destruct au_empty; iSteps.
+
+    - destruct au_empty.
+
+      + iDestruct "HΨ" as "(Hl_front_1 & HΨ)".
+        iDestruct (pointsto_agree with "Hl_front_1 Hl_front_2") as %[= ->].
+        iAssert ⌜length past = i⌝%I as %Hpast_length.
+        { iDestruct (node2_schain_NoDup with "Hhist") as %Hnodup.
+          iPureIntro. eapply NoDup_lookup; try done.
+          rewrite Hhist list_lookup_middle //.
+        }
+        destruct (decide (length vs = 0)) as [->%nil_length_inv | Hvs]; last first.
+        { iDestruct (big_sepL2_length with "Hnodes") as %?.
+          exfalso.
+          apply (f_equal length) in Hhist.
+          opose proof* lookup_last_length as Heq; [done.. |].
+          rewrite Heq app_length /= in Hhist. lia.
+        }
+        iMod "HΨ" as "(%vs & (%_l & %_γ & %Heq & #_Hmeta & Hmodel₁) & _ & HΨ)". injection Heq as <-.
+        iDestruct (meta_agree with "Hmeta _Hmeta") as %<-. iClear "_Hmeta".
+        iDestruct (mpsc_queue_model_agree with "Hmodel₁ Hmodel₂") as %->.
+        iDestruct ("Hβ_empty" with "[Hmodel₁]") as "Hβ"; first iSteps.
+        iMod ("HΨ" with "Hβ") as "HΨ".
+        iSplitR "Hl_front_1 HΨ HΦ". { repeat iExists _. iSteps. }
+        iSteps.
+
+      + iSplitR "HΦ". { repeat iExists _. iSteps. }
+        iSteps.
+  Qed.
+  #[local] Lemma mpsc_queue_node2_next_spec l γ ι i node :
+    {{{
+      meta l nroot γ ∗
+      inv ι (mpsc_queue_inv_inner l γ) ∗
+      mpsc_queue_history_elem γ i node
+    }}}
+      !#node.[node2_next]
+    {{{ res,
+      RET res;
+        ⌜res = ()%V⌝
+      ∨ ∃ node',
+        ⌜res = #node'⌝ ∗
+        mpsc_queue_history_elem γ (S i) node'
+    }}}.
+  Proof.
+    iIntros "%Φ (#Hmeta & #Hinv & #Hhistory_elem) HΦ".
+    wp_apply (mpsc_queue_node2_next_spec_strong false false TeleO inhabitant inhabitant inhabitant inhabitant with "[$Hmeta $Hinv $Hhistory_elem //]").
+    iSteps.
+  Qed.
+  #[local] Lemma mpsc_queue_node2_next_spec_au_empty TB β x Ψ l γ ι i node :
+    {{{
+      meta l nroot γ ∗
+      inv ι (mpsc_queue_inv_inner l γ) ∗
+      mpsc_queue_history_elem γ i node ∗
+      l.[front] ↦{#3/4} #node ∗
+      atomic_update (TA := [tele vs]) (TB := TB) (⊤ ∖ ↑ι) ∅ (tele_app $ mpsc_queue_model #l) β Ψ ∗
+      (mpsc_queue_model #l [] -∗ β [tele_arg []] x)
+    }}}
+      !#node.[node2_next]
+    {{{ res,
+      RET res;
+        ⌜res = ()%V⌝ ∗
+        l.[front] ↦{#3/4} #node ∗
+        Ψ [tele_arg []] x
+      ∨ ∃ node',
+        ⌜res = #node'⌝ ∗
+        mpsc_queue_history_elem γ (S i) node' ∗
+        l.[front] ↦{#3/4} #node ∗
+        atomic_update (TA := [tele vs]) (TB := TB) (⊤ ∖ ↑ι) ∅ (tele_app $ mpsc_queue_model #l) β Ψ
+    }}}.
+  Proof.
+    iIntros "%Φ (#Hmeta & #Hinv & #Hhistory_elem & Hl_front & HΨ & Hβ) HΦ".
+    wp_apply (mpsc_queue_node2_next_spec_strong true false _ _ _ x with "[$]").
+    iSteps.
+  Qed.
+  #[local] Lemma mpsc_queue_node2_next_spec_au TB β x_empty x_nonempty Ψ l γ ι i node :
+    {{{
+      meta l nroot γ ∗
+      inv ι (mpsc_queue_inv_inner l γ) ∗
+      mpsc_queue_history_elem γ i node ∗
+      l.[front] ↦{#3/4} #node ∗
+      atomic_update (TA := [tele vs]) (TB := TB) (⊤ ∖ ↑ι) ∅ (tele_app $ mpsc_queue_model #l) β Ψ ∗
+      ( mpsc_queue_model #l [] -∗
+        β [tele_arg []] x_empty
+      ) ∗
+      ( ∀ vs,
+        ⌜vs ≠ []⌝ -∗
+        mpsc_queue_model #l vs -∗
+        β (TeleArgCons vs ()) x_nonempty
+      )
+    }}}
+      !#node.[node2_next]
+    {{{ res,
+      RET res;
+        ⌜res = ()%V⌝ ∗
+        l.[front] ↦{#3/4} #node ∗
+        Ψ [tele_arg []] x_empty
+      ∨ ∃ node',
+        ⌜res = #node'⌝ ∗
+        mpsc_queue_history_elem γ (S i) node' ∗
+        l.[front] ↦{#3/4} #node ∗
+        ∃ vs, Ψ (TeleArgCons vs ()) x_nonempty
+    }}}.
+  Proof.
+    iIntros "%Φ (#Hmeta & #Hinv & #Hhistory_elem & Hl_front & HΨ & Hβ_empty & Hβ_nonempty) HΦ".
+    wp_apply (mpsc_queue_node2_next_spec_strong true true with "[$]").
+    iSteps.
+  Qed.
+
+  Lemma mpsc_queue_is_empty_spec t ι :
+    <<<
+      mpsc_queue_inv t ι ∗
+      mpsc_queue_consumer t
+    | ∀∀ vs,
+      mpsc_queue_model t vs
+    >>>
+      mpsc_queue_is_empty t @ ↑ι
+    <<<
+      mpsc_queue_model t vs
+    | RET #(bool_decide (vs = [])); True
+    >>>.
+  Proof.
+    iIntros "!> %Φ ((%l & %γ & -> & #Hmeta & #Hinv) & (%_l & %front & %Heq & Hl_front)) HΦ". injection Heq as <-.
+
+    iMod (mpsc_queue_inv_inner_history_elem with "Hinv Hl_front") as "(%i & Hl_front & #Hhistory_elem)".
+
+    iAssert (
+      AU <{
+        ∃∃ vs,
+        mpsc_queue_model #l vs
+      }> @ ⊤ ∖ ↑ι, ∅ <{
+        ∀∀ b,
+        ⌜b = bool_decide (vs = [])⌝ ∗
+        mpsc_queue_model #l vs
+      , COMM
+        True -∗ Φ #b
+      }>
+    )%I with "[HΦ]" as "HΦ".
+    { iAuIntro.
+      iApply (aacc_aupd_commit with "HΦ"); first done. iIntros "%vs Hmodel".
+      iAaccIntro with "Hmodel"; iSteps.
+    }
+
+    wp_rec. wp_load. wp_pures.
+    wp_smart_apply (mpsc_queue_node2_next_spec_au [tele_pair bool] _ [tele_arg true] [tele_arg false] with "[$Hmeta $Hinv $Hhistory_elem $Hl_front $HΦ]"); last iSteps.
+    iSplitR; iSteps.
+  Qed.
+
+  #[local] Lemma mpsc_queue_do_push_spec l γ ι i node new_back v :
+    <<<
+      meta l nroot γ ∗
+      inv ι (mpsc_queue_inv_inner l γ) ∗
+      mpsc_queue_history_elem γ i node ∗
+      node2_model new_back v ()
+    | ∀∀ vs,
+      mpsc_queue_model #l vs
+    >>>
+      mpsc_queue_do_push #node #new_back @ ↑ι
+    <<<
+      mpsc_queue_model #l (vs ++ [v])
+    | RET ();
+      ∃ j,
+      mpsc_queue_history_elem γ j new_back
+    >>>.
+  Proof.
+    iIntros "!> %Φ (#Hmeta & #Hinv & #Hhistory_elem & Hnew_back) HΦ".
+
+    iLöb as "HLöb" forall (i node) "Hhistory_elem".
+
+    wp_rec.
+    wp_smart_apply (mpsc_queue_node2_next_spec with "[$Hmeta $Hinv $Hhistory_elem]") as (res) "[-> | (%node' & -> & #Hhistory_elem')]"; last iSteps.
+    wp_pures.
+
+    wp_bind (Cas _ _ _).
+    iInv "Hinv" as "(%hist & %past & %front & %nodes & %back & %vs & >%Hhist & >%Hback & Hl_front & Hl_back & Hhist & Hnodes & >Hhistory_auth & Hmodel₂)".
+    iDestruct (mpsc_queue_history_agree with "Hhistory_auth Hhistory_elem") as %Hlookup.
+    iDestruct (node2_schain_lookup' with "Hhist") as "(Hhist1 & Hnode & Hhist2)"; first done.
+    destruct (hist !! S i) as [node' |] eqn:Hlookup'; simpl.
+
+    - wp_cas as _ | [] _.
+      iDestruct (node2_schain_lookup'_2 with "Hhist1 Hnode Hhist2") as "Hhist"; [done | rewrite Hlookup' // |].
+      iSplitR "Hnew_back HΦ". { repeat iExists _. iSteps. }
+      iSteps.
+
+    - wp_cas as Hcas | _ _; first done.
+      iDestruct (node2_schain_lookup'_2 with "Hhist1 Hnode []") as "Hhist"; [done | rewrite Hlookup' // | ..].
+      { rewrite -(lookup_last_length hist) // drop_all //. }
+      iDestruct "Hnew_back" as "(Hnew_back_data & Hnew_back_next)".
+      iDestruct (big_sepL2_snoc with "[$Hnodes $Hnew_back_data]") as "Hnodes".
+      iDestruct (node2_schain_snoc_2 with "Hhist Hnew_back_next") as "Hhist".
+      iMod (mpsc_queue_history_update new_back with "Hhistory_auth") as "Hhistory_auth".
+      iDestruct (mpsc_queue_history_elem_get with "Hhistory_auth") as "#Hhistory_elem_new_back".
+      { rewrite lookup_snoc_Some. naive_solver. }
+      iMod "HΦ" as "(%_vs & (%_l & %_γ & %Heq & #_Hmeta & Hmodel₁) & _ & HΦ)". injection Heq as <-.
+      iDestruct (meta_agree with "Hmeta _Hmeta") as %<-. iClear "_Hmeta".
+      iDestruct (mpsc_queue_model_agree with "Hmodel₁ Hmodel₂") as %->.
+      iMod (mpsc_queue_model_update (vs ++ [v]) with "Hmodel₁ Hmodel₂") as "(Hmodel₁ & Hmodel₂)".
+      iMod ("HΦ" with "[Hmodel₁]") as "HΦ"; [iSteps.. |].
+      iSplitR "HΦ".
+      { iExists (hist ++ [new_back]), past, front, (nodes ++ [new_back]), back, (vs ++ [v]).
+        iSteps; iPureIntro.
+        - rewrite Hhist -assoc //.
+        - rewrite elem_of_app. naive_solver.
+      }
+      iSteps.
+  Qed.
+
+  #[local] Lemma mpsc_queue_fix_back_spec l γ ι i back j new_back :
+    {{{
+      meta l nroot γ ∗
+      inv ι (mpsc_queue_inv_inner l γ) ∗
+      mpsc_queue_history_elem γ i back ∗
+      mpsc_queue_history_elem γ j new_back
+    }}}
+      mpsc_queue_fix_back #l #back #new_back
+    {{{
+      RET (); True
+    }}}.
+  Proof.
+    iIntros "%Φ (#Hmeta & #Hinv & #Hhistory_elem_back & #Hhistory_elem_new_back) HΦ".
+
+    iLöb as "HLöb" forall (i back) "Hhistory_elem_back".
+
+    wp_rec. wp_pures.
+    wp_bind (_ and _)%E.
+    wp_apply (wp_wand _ _ (λ res, ∃ b, ⌜res = #b⌝)%I) as (res) "(%b & ->)".
+    { wp_smart_apply (mpsc_queue_node2_next_spec with "[$Hmeta $Hinv $Hhistory_elem_new_back]") as (res) "[-> | (%new_back' & -> & #Hhistory_elem_new_back')]"; last iSteps.
+      wp_pures.
+
+      wp_bind (Cas _ _ _).
+      iInv "Hinv" as "(%hist & %past & %front & %nodes & %back' & %vs & >%Hhist & >%Hback & Hl_front & Hl_back & Hhist & Hnodes & Hhistory_auth & Hmodel₂)".
+      wp_cas as _ | -> _.
+      2: iDestruct (mpsc_queue_history_agree with "Hhistory_auth Hhistory_elem_new_back") as %Hnew_back%elem_of_list_lookup_2.
+      all: iSplitL; first (repeat iExists _; iSteps).
+      all: iSteps.
+    }
+    destruct b; last iSteps.
+    wp_smart_apply (mpsc_queue_back_spec with "Hinv") as (back' i') "#Hhistory_elem_back'".
+    iApply ("HLöb" with "HΦ Hhistory_elem_back'").
+  Qed.
 
   Lemma mpsc_queue_push_spec t ι v :
     <<<
@@ -135,7 +657,16 @@ Section mpsc_queue_G.
     | RET (); True
     >>>.
   Proof.
-  Admitted.
+    iIntros "!> %Φ (%l & %γ & -> & #Hmeta & #Hinv) HΦ".
+
+    wp_rec.
+    wp_smart_apply (node2_create_spec with "[//]") as (new_back) "Hnew_back".
+    wp_smart_apply (mpsc_queue_back_spec with "Hinv") as (back i) "#Hhistory_elem_back".
+    wp_smart_apply (mpsc_queue_do_push_spec with "[$Hmeta $Hinv $Hhistory_elem_back $Hnew_back]").
+    iApply (atomic_update_wand with "HΦ"). iIntros "%vs HΦ (%j & #Hhistory_elem_new_back)".
+    wp_smart_apply (mpsc_queue_fix_back_spec with "[$Hmeta $Hinv Hhistory_elem_back Hhistory_elem_new_back] HΦ").
+    iSteps.
+  Qed.
 
   Lemma mpsc_queue_pop_spec t ι :
     <<<
@@ -151,7 +682,44 @@ Section mpsc_queue_G.
       mpsc_queue_consumer t
     >>>.
   Proof.
-  Admitted.
+    iIntros "!> %Φ ((%l & %γ & -> & #Hmeta & #Hinv) & (%_l & %front & %Heq & Hl_front_1)) HΦ". injection Heq as <-.
+
+    iLöb as "HLöb".
+
+    iMod (mpsc_queue_inv_inner_history_elem with "Hinv Hl_front_1") as "(%i & Hl_front_1 & #Hhistory_elem)".
+
+    wp_rec. wp_load.
+    wp_smart_apply (mpsc_queue_node2_next_spec_au_empty _ _ [tele_arg] with "[$Hmeta $Hinv $Hhistory_elem $Hl_front_1 $HΦ]") as (res) "[(-> & Hl_front_1 & HΦ) | (%front' & -> & #Hhistory_elem' & Hl_front_1 & HΦ)]"; [iSteps.. |].
+    wp_pures.
+
+    wp_bind (_ <- _)%E.
+    iInv "Hinv" as "(%hist & %past & %_front & %nodes & %back & %vs & >%Hhist & >%Hback & >Hl_front_2 & Hl_back & Hhist & Hnodes & >Hhistory_auth & Hmodel₂)".
+    iDestruct (pointsto_agree with "Hl_front_1 Hl_front_2") as %[= <-].
+    iCombine "Hl_front_1 Hl_front_2" as "Hl_front".
+    rewrite Qp.three_quarter_quarter.
+    wp_store.
+    iEval (rewrite -Qp.three_quarter_quarter) in "Hl_front".
+    iDestruct "Hl_front" as "(Hl_front_1 & Hl_front_2)".
+    iDestruct (mpsc_queue_history_agree with "Hhistory_auth Hhistory_elem") as %Hlookup.
+    iDestruct (mpsc_queue_history_agree with "Hhistory_auth Hhistory_elem'") as %Hlookup'.
+    iAssert ⌜length past = i⌝%I as %Hpast_length.
+    { iDestruct (node2_schain_NoDup with "Hhist") as %Hnodup.
+      iPureIntro. eapply NoDup_lookup; try done.
+      rewrite Hhist list_lookup_middle //.
+    }
+    rewrite Hhist (assoc _ _ [_]) lookup_app_r app_length /= in Hlookup'; first lia.
+    rewrite Nat.add_1_r Hpast_length Nat.sub_diag in Hlookup'.
+    destruct nodes as [| node nodes]; first done. injection Hlookup' as ->.
+    rewrite (assoc _ _ [_]) in Hhist.
+    iDestruct (big_sepL2_cons_inv_l with "Hnodes") as "(%v & %vs' & -> & Hfront_data & Hnodes)".
+    iMod "HΦ" as "(%_vs & (%_l & %_γ & %Heq & #_Hmeta & Hmodel₁) & _ & HΦ)". injection Heq as <-.
+    iDestruct (meta_agree with "Hmeta _Hmeta") as %<-. iClear "_Hmeta".
+    iDestruct (mpsc_queue_model_agree with "Hmodel₁ Hmodel₂") as %->.
+    iMod (mpsc_queue_model_update vs' with "Hmodel₁ Hmodel₂") as "(Hmodel₁ & Hmodel₂)".
+    iMod ("HΦ" with "[Hmodel₁]") as "HΦ"; first iSteps.
+    iSplitR "Hl_front_1 Hfront_data HΦ". { repeat iExists _. iSteps. }
+    iSteps.
+  Qed.
 End mpsc_queue_G.
 
 #[global] Opaque mpsc_queue_create.
